\begin{statement}{1.2}
  Suppose that $a,m>0$, and $a \not\equiv 0\pmod m$, prove that
  \begin{equation*}
    (-a) \bmod m = m - (a \bmod m)
  \end{equation*}
\end{statement}
\begin{proof}

  Let $r = a \bmod m$. This means there is a $q$ such that $a = qm + r$. So:
  \begin{eqnarray*}
    (-a) \bmod m &=& (-qm - r) \bmod m \\
    &=& (-(q+1)m + m - r ) \bmod m
  \end{eqnarray*}

  Since $a \not\equiv 0 \pmod m$, it is true that $r \in [1,m-1]$, so $0 < m - r < m$. Thus:

    \begin{eqnarray*}
      (-(q+1)m + m - r ) \bmod m &=&  m - r \\
      &=& m - (a \bmod m)
    \end{eqnarray*}

  
\end{proof}
